projection/endpoint_to_payloadScript.sml
@@ -4,7 +4,7 @@ val _ = new_theory "endpoint_to_payload";
 
 val compile_endpoint_def = Define `
    (compile_endpoint endpointLang$Nil = payloadLang$Nil)
-∧ (compile_endpoint (Send p v e) = Send p (INL v) (compile_endpoint e))
+∧ (compile_endpoint (Send p v e) = Send p v 0 (compile_endpoint e))
 ∧ (compile_endpoint (Receive p v e) = Receive p v [] (compile_endpoint e))
 ∧ (compile_endpoint (IntChoice b p e) = IntChoice b p (compile_endpoint e))
 ∧ (compile_endpoint (ExtChoice p e1 e2) = ExtChoice p (compile_endpoint e1) (compile_endpoint e2))
